Switch to execCrash for basic crash definition
No longer define execHalt for halt execution; crash step is always
chained on. This is a nice simplification since in practice we always
had a crash afterward, and the paper's exposition and equations benefits
greatly from combining the two.

CHL now uses crash specs in the correct sense (rather than FSCQ's halt
specs that are called crash specs).

src/Spec/Hoare.v
@@ -33,17 +33,6 @@ Definition spec_impl
             (forall s' rv, (spec1 s).(alternate) s' rv ->
                            (spec2 s).(alternate) s' rv).
 
-Definition op_spec `(sem: Dynamics Op State) `(op : Op T) : Specification T unit State :=
-  fun state =>
-    {|
-      pre := True;
-      post :=
-        fun state' v => sem.(step) op state state' v;
-      alternate :=
-        fun state' r =>
-          r = tt /\ (state' = state \/ exists v, sem.(step) op state state' v);
-    |}.
-
 Definition op_cstep_spec `(sem: Dynamics Op State) `(op : Op T) : Specification T unit State :=
   fun state =>
     {|
@@ -61,7 +50,7 @@ Section Hoare.
   Context `(sem: Dynamics Op State).
   Notation proc := (proc Op).
   Notation exec := sem.(exec).
-  Notation exec_halt := sem.(exec_halt).
+  Notation exec_crash := sem.(exec_crash).
   Notation crash_step := sem.(crash_step).
   Notation rexec := sem.(rexec).
 
@@ -75,7 +64,7 @@ Section Hoare.
              (p: proc T)
              (spec: Specification T unit State) :=
     exec p ---> spec_exec spec /\
-    exec_halt p ---> spec_aexec spec.
+    exec_crash p ---> spec_aexec spec.
 
   Theorem proc_rspec_expand T R
           (p: proc T) (rec: proc R)
@@ -102,7 +91,7 @@ Section Hoare.
       (spec s).(pre) ->
       (forall s' v, exec p s s' v ->
                (spec s).(post) s' v) /\
-      (forall s' rv, exec_halt p s s' rv ->
+      (forall s' rv, exec_crash p s s' rv ->
                 (spec s).(alternate) s' rv).
   Proof.
     unfold proc_hspec, rimpl, spec_exec, spec_aexec; split; intros.
@@ -185,7 +174,7 @@ Section Hoare.
       specialize (Hok t). rewrite proc_rspec_expand in Hok.
       destruct (Hok state_mid) as (Hrx_ok&Hrx_rec); simpl; eauto.
     - rewrite rexec_unfold. rewrite rexec_unfold in Hp_rec.
-      simpl. rewrite exec_halt_idem, bind_dist_r.
+      simpl. rewrite bind_dist_r.
       apply rel_or_elim.
       + rewrite Hp_rec; auto.
         intros state state' r Hspec_aexec Hpre'.
@@ -225,7 +214,7 @@ Section Hoare.
       specialize (Hrx _ Hpre') as (Hpre&Hok&Hrec).
       specialize (Hok t). rewrite proc_hspec_expand in Hok.
       destruct (Hok state_mid) as (Hrx_ok&Hrx_rec); simpl; eauto.
-    - simpl. rewrite exec_halt_idem.
+    - simpl.
       apply rel_or_elim.
       + rewrite Hp_rec; auto.
         intros state state' r Hspec_aexec Hpre'.
@@ -294,12 +283,14 @@ Section Hoare.
           (v:T):
     (forall state, pre (spec state) ->
                      post (spec state) state v /\
-                     alternate (spec state) state tt) ->
+                     (forall state', crash_step state state' tt -> alternate (spec state) state' tt)) ->
     proc_hspec (Ret v) spec .
   Proof.
-    unfold proc_hspec; intros Himpl; split;
-    intros state state' t Hexec Hpre;
-    inversion Hexec; subst; specialize (Himpl _ Hpre); intuition.
+    unfold proc_hspec, spec_exec, spec_aexec; simpl.
+    unfold "--->", pure; split; propositional.
+    specialize (H _ H1); propositional.
+    specialize (H _ H1); propositional.
+    destruct o; eauto.
   Qed.
 
   (** Define what it means for a spec to be idempotent: *)
@@ -319,11 +310,10 @@ Section Hoare.
   Definition idempotent_crash_step A T R `(spec: A -> Specification T R State) :=
     forall a state,
       pre (spec a state) ->
-      forall v state' state'', alternate (spec a state) state' v ->
-                               crash_step state' state'' tt ->
-               exists a', pre (spec a' state'') /\
-                    forall rv state''', post (spec a' state'') state''' rv ->
-                                  post (spec a state) state''' rv.
+      forall v state', alternate (spec a state) state' v ->
+               exists a', pre (spec a' state') /\
+                    forall rv state'', post (spec a' state') state'' rv ->
+                                  post (spec a state) state'' rv.
 
   (** In some situations, the precondition of a specification
     may define variables or facts that you want to [intros].
@@ -371,21 +361,20 @@ Section Hoare.
   Qed.
 
   Theorem op_spec_sound T (op: Op T):
-    proc_hspec (Call op) (op_spec sem op).
+    proc_hspec (Call op) (op_cstep_spec sem op).
   Proof.
     unfold proc_hspec; split.
     - intros state state' t Hexec Hpre; eauto.
     - simpl. apply rel_or_elim.
       * intros s s' [] Hl Hpre. simpl. split; auto.
-        firstorder.
       * intros s s' [] Hl Hpre.
-        inversion Hl as (?&?&?&Hrest). inversion Hrest; subst.
+        inversion Hl as (?&?&?&Hrest).
         firstorder.
   Qed.
 
   Theorem op_spec_complete T (op: Op T):
-    spec_exec (op_spec sem op) ---> exec (Call op) /\
-    spec_aexec (op_spec sem op) ---> exec_halt (Call op).
+    spec_exec (op_cstep_spec sem op) ---> exec (Call op) /\
+    spec_aexec (op_cstep_spec sem op) ---> exec_crash (Call op).
   Proof. split; firstorder. Qed.
 
   Theorem op_cstep_spec_complete1 T (op: Op T):
@@ -420,12 +409,11 @@ Section Hoare.
     (forall s, (p_rspec s).(pre) -> (p_hspec s).(pre) /\
                (forall s' v, (p_hspec s).(post) s' v ->
                              (p_rspec s).(post) s' v)) ->
-    (* alternate of hspec followed by crash implies pre of rec for some ghost*)
-    (forall state state' state'' v,
+    (* alternate of hspec implies pre of rec for some ghost*)
+    (forall state state' v,
         pre (p_hspec state) ->
         alternate (p_hspec state) state' v ->
-        crash_step state' state'' tt ->
-        exists a, pre (rec_hspec a state'')) ->
+        exists a, pre (rec_hspec a state')) ->
     (* recovery post implies alternate of rspec *)
     (forall a s sc, (p_rspec s).(pre) ->
                     (forall sfin rv, (rec_hspec a sc).(post) sfin rv ->
@@ -447,13 +435,12 @@ Section Hoare.
       intros s1 [].
 
       setoid_rewrite <-bind_assoc.
-      assert (_ <- test (fun s' : State => (p_hspec s1).(pre) /\ (p_hspec s1).(alternate) s' tt); crash_step
+      assert (test (fun s' : State => (p_hspec s1).(pre) /\ (p_hspec s1).(alternate) s' tt)
               ---> @any _ _ unit ;; test (fun s' : State => exists a', (rec_hspec a' s').(pre)))
         as HCI.
       {
-        intros s s' [] ([]&?&(((Hpre&Halt)&?)&Hcrash)); subst.
-        unfold any; exists tt; eexists; split; auto.
-        split; eauto.
+        unfold test, rimpl, any; propositional.
+        exists tt; eexists; intuition eauto.
       }
       rew HCI.
 
@@ -468,10 +455,9 @@ Section Hoare.
         subst. eapply Hr_alt; eauto.
         eapply Hc; eauto.
       * intros s s' [] Hl.
-        destruct Hl as ([]&?&((a'&Hhspec)&<-)&Hexec_halt).
+        destruct Hl as ([]&?&((a'&Hhspec)&<-)&Hexec_crash).
         unfold any; exists tt; eexists; split; auto.
         split; [| eauto].
-        destruct Hexec_halt as ([]&smid&Hexec_halt&Hcrash_step).
         edestruct Hidemp as (a''&?); eauto.
         eapply Hc; eauto. eexists; intuition eauto.
       * apply any_seq_star_any.
