src/Spec/ProcTheorems.v
@@ -13,15 +13,15 @@ Section Dynamics.
   Notation proc := (proc Op).
   Notation step := sem.(step).
   Notation crash_step := sem.(crash_step).
-  Notation exec_halt := sem.(exec_halt).
+  Notation exec_crash := sem.(exec_crash).
   Notation exec := sem.(exec).
   Notation exec_recover := sem.(exec_recover).
   Notation rexec := sem.(rexec).
 
   Hint Resolve rimpl_refl requiv_refl : core.
 
-  Theorem exec_halt_finish T (p: proc T) :
-    exec p;; pure tt ---> exec_halt p.
+  Theorem exec_crash_finish T (p: proc T) :
+    exec p;; crash_step ---> exec_crash p.
   Proof.
     induction p; simpl in *; norm.
     - rewrite <- rel_or_intror.
@@ -31,29 +31,30 @@ Section Dynamics.
       eauto.
   Qed.
 
-  Theorem exec_halt_noop T (p: proc T) :
-    pure tt ---> exec_halt p.
+  Theorem exec_crash_noop T (p: proc T) :
+    crash_step ---> exec_crash p.
   Proof.
     induction p; simpl in *; norm.
-    - rewrite <- rel_or_introl; auto.
-    - rewrite <- rel_or_introl, <- rel_or_introl; auto.
+    - Left.
+    - Left.
+      auto.
   Qed.
 
-  Theorem exec_halt_ret T (v: T) :
-    exec_halt (Ret v) <---> pure tt.
+  Theorem exec_crash_ret T (v: T) :
+    exec_crash (Ret v) <---> crash_step.
   Proof.
     reflexivity.
   Qed.
 
-  Theorem exec_halt_idem T (p: proc T) :
-    pure tt + exec_halt p <---> exec_halt p.
+  Theorem exec_crash_idem T (p: proc T) :
+    crash_step + exec_crash p <---> exec_crash p.
   Proof.
-    apply rimpl_or; auto using exec_halt_noop.
+    apply rimpl_or; auto using exec_crash_noop.
   Qed.
 
   Definition exec_equiv T (p p': proc T) :=
     exec p <---> exec p' /\
-    exec_halt p <---> exec_halt p'.
+    exec_crash p <---> exec_crash p'.
 
   Global Instance exec_equiv_equiv T : Equivalence (exec_equiv (T:=T)).
   Proof.
@@ -85,8 +86,8 @@ Section Dynamics.
     Proper (@exec_equiv T ==> @requiv State State T) exec.
   Proof. intros ?? (?&?); intuition. Qed.
 
-  Global Instance exec_halt_respectful T:
-    Proper (@exec_equiv T ==> @requiv State State unit) exec_halt.
+  Global Instance exec_crash_respectful T:
+    Proper (@exec_equiv T ==> @requiv State State unit) exec_crash.
   Proof. intros ?? (?&?); intuition. Qed.
 
   Global Instance rexec_respectful T R:
@@ -97,8 +98,7 @@ Section Dynamics.
       Bind (Ret v) p <==> p v.
   Proof.
     split; simpl; norm.
-    rew rel_or_idem.
-    rew exec_halt_idem.
+    rew exec_crash_idem.
   Qed.
 
   Theorem monad_assoc
@@ -108,8 +108,6 @@ Section Dynamics.
     Bind (Bind p1 p2) p3 <==> Bind p1 (fun v => Bind (p2 v) p3).
   Proof.
     split; simpl; norm.
-    rew rel_or_idem.
-    rew exec_halt_idem.
     repeat setoid_rewrite bind_dist_l.
     norm.
   Qed.
@@ -124,11 +122,10 @@ Section Dynamics.
   Proof.
     repeat unfold exec_recover, rexec; simpl; norm.
 
-    rewrite exec_halt_idem.
     rewrite ?bind_dist_r; norm.
 
     (* a few abstractions *)
-    gen (exec rec1) (exec_halt rec1) crash_step;
+    gen (exec rec1) (exec_crash rec1) crash_step;
       clear rec1;
       intros rec1 rec1_crash crash.
 
@@ -145,7 +142,6 @@ Section Dynamics.
   Proof.
     unfold rexec, exec_recover.
     setoid_rewrite <- bind_assoc at 1.
-    setoid_rewrite <- bind_assoc at 1.
     rew seq_star1.
   Qed.
 
@@ -154,24 +150,24 @@ Section Dynamics.
     crash_step;; exec_recover rec ---> rexec rec rec.
   Proof.
     unfold rexec, exec_recover.
-    setoid_rewrite <- exec_halt_noop at 2; norm.
+    setoid_rewrite <- exec_crash_noop at 2; norm.
   Qed.
 
-  Lemma exec_halt_ret_proc `(rec: proc R):
-    exec_halt (Ret tt) ---> exec_halt rec.
+  Lemma exec_crash_ret_proc `(rec: proc R):
+    exec_crash (Ret tt) ---> exec_crash rec.
   Proof. induction rec; simpl; firstorder. Qed.
 
-  Lemma exec_halt_ret_recover_fold `(rec: proc R):
-    _ <- exec_halt (Ret tt); _ <- crash_step; exec_recover rec ---> exec_recover rec.
+  Lemma exec_crash_ret_recover_fold `(rec: proc R):
+    _ <- exec_crash (Ret tt); exec_recover rec ---> exec_recover rec.
   Proof.
-    setoid_rewrite (exec_halt_ret_proc rec).
+    setoid_rewrite (exec_crash_ret_proc rec).
     unfold exec_recover.
-    do 2 setoid_rewrite <-bind_assoc.
+    setoid_rewrite <-bind_assoc.
     rewrite seq_star_fold; eauto.
   Qed.
 
 End Dynamics.
 
-Arguments exec_halt_noop [Op State sem T].
-Arguments exec_halt_finish [Op State sem T].
-Arguments exec_halt_ret [Op State sem T].
+Arguments exec_crash_noop [Op State sem T].
+Arguments exec_crash_finish [Op State sem T].
+Arguments exec_crash_ret [Op State sem T].
